

تمرین ۱

قرار است برای دو متغیر تصادفی X و Y ثابت شود:

$$\text{Var}(X + Y) = \text{Var}(X) + \text{Var}(Y) + 2 \text{Cov}(X, Y)$$

definition: the from start We

$$\text{Var}(X) = \mathbb{E}[X^2] - (\mathbb{E}[X])^2$$

find: to want We

$$\text{Var}(X + Y)$$

definition: By

$$\text{Var}(X + Y) = \mathbb{E}[(X + Y)^2] - (\mathbb{E}[X + Y])^2$$

expectation: of linearity Using

$$\mathbb{E}[X + Y] = \mathbb{E}[X] + \mathbb{E}[Y]$$

square: the expanding and

$$(X + Y)^2 = X^2 + 2XY + Y^2$$

So,

$$\mathbb{E}[(X + Y)^2] = \mathbb{E}[X^2 + 2XY + Y^2] = \mathbb{E}[X^2] + 2\mathbb{E}[XY] + \mathbb{E}[Y^2]$$

Also,

$$(\mathbb{E}[X + Y])^2 = (\mathbb{E}[X] + \mathbb{E}[Y])^2 = (\mathbb{E}[X])^2 + 2\mathbb{E}[X]\mathbb{E}[Y] + (\mathbb{E}[Y])^2$$

back: Substituting

$$\begin{aligned} \text{Var}(X + Y) &= (\mathbb{E}[X^2] + 2\mathbb{E}[XY] + \mathbb{E}[Y^2]) - ((\mathbb{E}[X])^2 + 2\mathbb{E}[X]\mathbb{E}[Y] + (\mathbb{E}[Y])^2) \\ &= \underbrace{(\mathbb{E}[X^2] - (\mathbb{E}[X])^2)}_{\text{Var}(X)} + \underbrace{(\mathbb{E}[Y^2] - (\mathbb{E}[Y])^2)}_{\text{Var}(Y)} + 2 \underbrace{(\mathbb{E}[XY] - \mathbb{E}[X]\mathbb{E}[Y])}_{\text{Cov}(X,Y)} \end{aligned}$$

$$\text{Var}(X + Y) = \text{Var}(X) + \text{Var}(Y) + 2 \text{Cov}(X, Y)$$

$$\sum_{n=1}^8 \alpha_1^8 \cap \cup \quad (1)$$

model	MSE	MAE
regression	۱۱	۱۲
ridge	۱۳	۱۴
lasso	۱۵	۱۵

Table :۱ Caption



Caption :۱ شکل